cryptis/primitives/with_cryptis_spec.v
@@ -1,0 +1,635 @@
+From cryptis Require Import lib.
+From mathcomp Require Import ssreflect.
+From mathcomp Require order.
+From stdpp Require Import gmap.
+From iris.algebra Require Import agree auth gset gmap reservation_map.
+From iris.base_logic.lib Require Import invariants saved_prop.
+From iris.program_logic Require Import atomic.
+From iris.heap_lang Require Import notation proofmode.
+From iris.heap_lang.lib Require Import nondet_bool ticket_lock.
+From cryptis Require Import term cryptis.
+From cryptis.core Require Import minted_spec.
+From cryptis.primitives Require Import notations pre_term comp simple with_cryptis.
+From reloc Require Import reloc.
+
+Set Implicit Arguments.
+Unset Strict Implicit.
+Unset Printing Implicit Defensive.
+
+Local Existing Instance cryptisGS_tlock.
+Local Existing Instance ticket_lock.
+
+Section Proofs.
+
+Context `{!relocG Σ, !minted_specGS Σ}.
+
+Notation nonce := loc.
+Implicit Types E : coPset.
+Implicit Types a : nonce.
+Implicit Types t : term.
+Implicit Types v : val.
+Implicit Types Φ : prodO locO termO -n> iPropO Σ.
+Implicit Types Ψ : val → iProp Σ.
+
+Lemma twp_mk_nonce_gen E j :
+  ↑minted_specN ⊆ E →
+  nclose specN ⊆ E →
+  minted_spec_ctx -∗
+  refines_right j (mk_nonce #()) -∗
+  |={E}=> ∃ t, refines_right j t ∗ ⌜is_nonce t⌝ ∗
+               ((minted_spec t -∗ False) ∧ (|==> minted_spec t)).
+Proof.
+iIntros "% % #minted j"; rewrite /mk_nonce.
+tp_pures j.
+tp_alloc j as a "Ha".
+tp_pures j.
+iExists (TNonce a).
+rewrite val_of_term_unseal. iFrame. iModIntro.  iSplit => //.
+
+
+rewrite /mk_nonce; iIntros "mint post".
+wp_pures; wp_bind (ref _)%E; iApply twp_alloc=> //.
+iIntros (a) "[_ token]".
+iPoseProof (nonce_alloc P Q with "token") as "fresh".
+iPoseProof ("mint" with "fresh") as ">(#? & #? & #? & ?)".
+iSpecialize ("post" $! (TNonce a)).
+wp_pures. rewrite val_of_term_unseal /=.
+iApply ("post" with "[] [] [] [$]"); eauto.
+Qed.
+
+Lemma wp_mk_nonce_gen (P Q : term → iProp Σ) E Ψ (Φ : term → iProp Σ) :
+  (∀ t, (minted t -∗ False) ∧
+        (|==> minted t ∗
+              □ (public t ↔ ▷ □ P t) ∗
+              □ (∀ t', dh_pred t t' ↔ ▷ □ Q t')) ={E}=∗
+        minted t ∗
+        □ (public t ↔ ▷ □ P t) ∗
+        □ (∀ t', dh_pred t t' ↔ ▷ □ Q t') ∗
+        Φ t) -∗
+  (∀ t, ⌜is_nonce t⌝ -∗
+        minted t -∗
+        □ (public t ↔ ▷ □ P t) -∗
+        □ (∀ t', dh_pred t t' ↔ ▷ □ Q t') -∗
+        Φ t -∗
+        Ψ t) -∗
+  WP mk_nonce #()%V @ E {{ Ψ }}.
+Proof.
+iIntros "H1 H2". iApply twp_wp.
+iApply (twp_mk_nonce_gen with "H1 H2").
+Qed.
+
+Lemma twp_mk_nonce_freshN (T : gset term) (P Q : term → iProp Σ) (T' : term → gset term) Ψ :
+  cryptis_ctx -∗
+  (∀ t, ⌜t ∈ T⌝ -∗ minted t) -∗
+  (∀ t, [∗ set] t' ∈ T' t, □ (minted t ↔ minted t')) -∗
+  (∀ t, ⌜∀ t', t' ∈ T → ¬ subterm t t'⌝ -∗
+        ⌜is_nonce t⌝ -∗
+        minted t -∗
+        □ (public t ↔ ▷ □ P t) -∗
+        □ (∀ t', dh_pred t t' ↔ ▷ □ Q t') -∗
+        ([∗ set] t' ∈ T' t, term_token t' ⊤) -∗
+        Ψ t) -∗
+  WP mk_nonce #()%V [{ Ψ }].
+Proof.
+iIntros "#ctx minted_T #minted_T' post".
+iApply (twp_mk_nonce_gen P Q ⊤ _
+          (λ t, ⌜∀ t', t' ∈ T → ¬ subterm t t'⌝ ∗
+          [∗ set] t' ∈ T' t, term_token t' ⊤)%I
+         with "[minted_T] [post]").
+{ iIntros "%t fresh".
+  iAssert (⌜∀ t', t' ∈ T → ¬ subterm t t'⌝)%I as "%fresh".
+  { iIntros "%t' %t'_T %t_t'".
+    iPoseProof ("minted_T" $! t' with "[//]") as "#minted_t'".
+    iPoseProof (subterm_minted t_t' with "minted_t'") as "minted_t".
+    iDestruct "fresh" as "[fresh _]".
+    by iApply "fresh". }
+  iMod (term_token_alloc (T' t)
+          (minted t -∗ False)
+          (minted t ∗ □ (public t ↔ ▷ □ P t) ∗
+           □ (∀ t', dh_pred t t' ↔ ▷ □ Q t'))
+          with "ctx [] [] [fresh]") as "(post & token)" => //.
+  - iIntros "%t' %t'_t contra minted_t'". iApply "contra".
+    iSpecialize ("minted_T'" $! t).
+    rewrite big_sepS_delete //.
+    iDestruct "minted_T'" as "[#e _]". by iApply "e".
+  - iIntros "%t' %t'_t (minted_t & _)".
+    iSpecialize ("minted_T'" $! t).
+    rewrite big_sepS_delete //.
+    iDestruct "minted_T'" as "[#e _]". by iApply "e".
+  - iSplit.
+    + by iDestruct "fresh" as "[fresh _]".
+    + by iDestruct "fresh" as "[_ >fresh]".
+  iFrame. do !iModIntro.
+  iDestruct "post" as "(? & ? & ?)". eauto. }
+iIntros "% ? ? ? ? [? ?]".
+iApply ("post" with "[$] [$] [$] [$] [$] [$]").
+Qed.
+
+Lemma wp_mk_nonce_freshN (T : gset term) P Q (T' : term → gset term) Ψ :
+  cryptis_ctx -∗
+  (∀ t, ⌜t ∈ T⌝ -∗ minted t) -∗
+  (∀ t, [∗ set] t' ∈ T' t, □ (minted t ↔ minted t')) -∗
+  (∀ t, ⌜∀ t', t' ∈ T → ¬ subterm t t'⌝ -∗
+        ⌜is_nonce t⌝ -∗
+        minted t -∗
+        □ (public t ↔ ▷ □ P t) -∗
+        □ (∀ t', dh_pred t t' ↔ ▷ □ Q t') -∗
+        ([∗ set] t' ∈ T' t, term_token t' ⊤) -∗
+        Ψ t) -∗
+  WP mk_nonce #()%V {{ Ψ }}.
+Proof.
+iIntros "#ctx H1 H2 H3".
+by iApply twp_wp; iApply (twp_mk_nonce_freshN with "[//] H1 H2 H3").
+Qed.
+
+Lemma twp_mk_nonce_fresh (T : gset term) (P Q : term → iProp Σ) Ψ :
+  cryptis_ctx -∗
+  (∀ t, ⌜t ∈ T⌝ -∗ minted t) -∗
+  (∀ t, ⌜∀ t', t' ∈ T → ¬ subterm t t'⌝ -∗
+        ⌜is_nonce t⌝ -∗
+        minted t -∗
+        □ (public t ↔ ▷ □ P t) -∗
+        □ (∀ t', dh_pred t t' ↔ ▷ □ Q t') -∗
+        term_token t ⊤ -∗
+        Ψ t) -∗
+  WP mk_nonce #()%V [{ Ψ }].
+Proof.
+iIntros "#ctx minted_T post".
+iApply (twp_mk_nonce_freshN T P Q (λ t : term, {[t]}) _
+         with "[//] minted_T [] [post]") => //.
+{ iIntros "%t". rewrite big_sepS_singleton. iModIntro.
+  iSplit; by iIntros "?". }
+iIntros "% ? ? ? ? ?".
+rewrite big_sepS_singleton.
+by iApply ("post" with "[$] [$] [$] [$] [$]").
+Qed.
+
+Lemma wp_mk_nonce_fresh (T : gset term) P Q Ψ :
+  cryptis_ctx -∗
+  (∀ t, ⌜t ∈ T⌝ -∗ minted t) -∗
+  (∀ t, ⌜∀ t', t' ∈ T → ¬ subterm t t'⌝ -∗
+        ⌜is_nonce t⌝ -∗
+        minted t -∗
+        □ (public t ↔ ▷ □ P t) -∗
+        □ (∀ t', dh_pred t t' ↔ ▷ □ Q t') -∗
+        term_token t ⊤ -∗
+        Ψ t) -∗
+  WP mk_nonce #()%V {{ Ψ }}.
+Proof.
+iIntros "#ctx H1 H2".
+by iApply twp_wp; iApply (twp_mk_nonce_fresh with "[//] H1 H2").
+Qed.
+
+Lemma twp_mk_nonce (P Q : term → iProp Σ) Ψ :
+  cryptis_ctx -∗
+  (∀ t, ⌜is_nonce t⌝ -∗
+        minted t -∗
+        □ (public t ↔ ▷ □ P t) -∗
+        □ (∀ t', dh_pred t t' ↔ ▷ □ Q t') -∗
+        term_token t ⊤ -∗
+        Ψ t) -∗
+  WP mk_nonce #()%V [{ Ψ }].
+Proof.
+iIntros "#ctx post". iApply (twp_mk_nonce_fresh ∅ P Q) => //.
+- iIntros "%". rewrite elem_of_empty. iDestruct 1 as "[]".
+- iIntros "% _". iApply "post".
+Qed.
+
+Lemma wp_mk_nonce (P Q : term → iProp Σ) Ψ :
+  cryptis_ctx -∗
+  (∀ t, ⌜is_nonce t⌝ -∗
+        minted t -∗
+        □ (public t ↔ ▷ □ P t) -∗
+        □ (∀ t', dh_pred t t' ↔ ▷ □ Q t') -∗
+        term_token t ⊤ -∗
+        Ψ t) -∗
+  WP mk_nonce #()%V {{ Ψ }}.
+Proof.
+iIntros "#ctx H".
+by iApply twp_wp; iApply (twp_mk_nonce with "[//] H").
+Qed.
+
+Lemma twp_mk_aenc_key Ψ :
+  cryptis_ctx -∗
+  (∀ sk : aenc_key,
+      minted sk -∗
+      secret sk -∗
+      term_token sk ⊤ -∗
+      Ψ sk) -∗
+  WP mk_aenc_key #() [{ Ψ }].
+Proof.
+iIntros "#ctx post". iMod unknown_alloc as (γ) "unknown".
+rewrite /mk_aenc_key. wp_pures.
+wp_bind (mk_nonce _).
+iApply (twp_mk_nonce_freshN ∅ (λ _, known γ 1) (λ _, False%I)
+  (λ t, {[(AEncKey t) : term]})) => //.
+- iIntros "% ?". by rewrite elem_of_empty.
+- iIntros "%t". rewrite [term_of_aenc_key]unlock big_sepS_singleton minted_TKey.
+  iModIntro. by iSplit; iIntros "?".
+iIntros "%t %fresh % #m_t #s_t _ token".
+rewrite big_sepS_singleton.
+pose sk := AEncKey t.
+iAssert (public sk ↔ ▷ □ known γ 1)%I as "s_sk".
+{ by rewrite public_adec_key. }
+iAssert (secret sk) with "[unknown]" as "tP"; first do 2?iSplit.
+- iMod (known_alloc with "unknown") as "#known".
+  by iSpecialize ("s_sk" with "known").
+- iMod (known_alloc 2 with "unknown") as "#known".
+  iIntros "!> !>". iSplit.
+  + iIntros "#p_sk".
+    iPoseProof ("s_sk" with "p_sk") as ">#known'".
+    by iPoseProof (known_agree with "known known'") as "%".
+  + iIntros "#contra".
+    iApply "s_sk". by iDestruct "contra" as ">[]".
+- iIntros "#p_sk".
+  iPoseProof ("s_sk" with "p_sk") as ">#known".
+  by iPoseProof (unknown_known with "[$] [//]") as "[]".
+wp_pures. wp_lam. iApply twp_key.
+rewrite [term_of_aenc_key]unlock /=.
+iApply ("post" $! (AEncKey _) with "[] [$] [$]").
+by rewrite minted_TKey.
+Qed.
+
+Lemma wp_mk_aenc_key Ψ :
+  cryptis_ctx -∗
+  (∀ sk : aenc_key,
+      minted sk -∗
+      secret sk -∗
+      term_token sk ⊤ -∗
+      Ψ sk) -∗
+  WP mk_aenc_key #() {{ Ψ }}.
+Proof.
+iIntros "#? ?". iApply twp_wp. by wp_apply twp_mk_aenc_key.
+Qed.
+
+Lemma twp_mk_sign_key Ψ :
+  cryptis_ctx -∗
+  (∀ sk : sign_key,
+      minted sk -∗
+      secret sk -∗
+      term_token sk ⊤ -∗
+      Ψ sk) -∗
+  WP mk_sign_key #() [{ Ψ }].
+Proof.
+iIntros "#ctx post". iMod unknown_alloc as (γ) "unknown".
+rewrite /mk_sign_key. wp_pures.
+wp_bind (mk_nonce _).
+iApply (twp_mk_nonce_freshN ∅ (λ _, known γ 1) (λ _, False%I)
+  (λ t, {[(SignKey t) : term]})) => //.
+- iIntros "% ?". by rewrite elem_of_empty.
+- iIntros "%t". rewrite [term_of_sign_key]unlock big_sepS_singleton minted_TKey.
+  iModIntro. by iSplit; iIntros "?".
+iIntros "%t %fresh % #m_t #s_t _ token".
+rewrite big_sepS_singleton.
+pose sk := SignKey t.
+iAssert (public sk ↔ ▷ □ known γ 1)%I as "s_sk".
+{ by rewrite public_sign_key. }
+iAssert (secret sk) with "[unknown]" as "tP"; first do 2?iSplit.
+- iMod (known_alloc with "unknown") as "#known".
+  by iSpecialize ("s_sk" with "known").
+- iMod (known_alloc 2 with "unknown") as "#known".
+  iIntros "!> !>". iSplit.
+  + iIntros "#p_sk".
+    iPoseProof ("s_sk" with "p_sk") as ">#known'".
+    by iPoseProof (known_agree with "known known'") as "%".
+  + iIntros "#contra".
+    iApply "s_sk". by iDestruct "contra" as ">[]".
+- iIntros "#p_sk".
+  iPoseProof ("s_sk" with "p_sk") as ">#known".
+  by iPoseProof (unknown_known with "[$] [//]") as "[]".
+wp_pures. wp_lam. iApply twp_key.
+rewrite [term_of_sign_key]unlock /=.
+iApply ("post" $! (SignKey _) with "[] [$] [$]").
+by rewrite minted_TKey.
+Qed.
+
+Lemma wp_mk_sign_key Ψ :
+  cryptis_ctx -∗
+  (∀ sk : sign_key,
+      minted sk -∗
+      secret sk -∗
+      term_token sk ⊤ -∗
+      Ψ sk) -∗
+  WP mk_sign_key #() {{ Ψ }}.
+Proof.
+iIntros "#? ?". iApply twp_wp. by wp_apply twp_mk_sign_key.
+Qed.
+
+Lemma twp_mk_senc_key Ψ :
+  cryptis_ctx -∗
+  (∀ k : senc_key,
+      minted k -∗
+      secret k -∗
+      term_token k ⊤ -∗
+      Ψ k) -∗
+  WP mk_senc_key #() [{ Ψ }].
+Proof.
+iIntros "#ctx post". iMod unknown_alloc as (γ) "unknown".
+rewrite /mk_senc_key. wp_pures.
+wp_bind (mk_nonce _).
+iApply (twp_mk_nonce_freshN ∅ (λ _, known γ 1) (λ _, False%I)
+  (λ t, {[(SEncKey t) : term]})) => //.
+- iIntros "% ?". by rewrite elem_of_empty.
+- iIntros "%t". rewrite [term_of_senc_key]unlock big_sepS_singleton minted_TKey.
+  iModIntro. by iSplit; iIntros "?".
+iIntros "%t %fresh % #m_t #s_t _ token".
+rewrite big_sepS_singleton.
+pose sk := SEncKey t.
+iAssert (public sk ↔ ▷ □ known γ 1)%I as "s_sk".
+{ by rewrite public_senc_key. }
+iAssert (secret sk) with "[unknown]" as "tP"; first do 2?iSplit.
+- iMod (known_alloc with "unknown") as "#known".
+  by iSpecialize ("s_sk" with "known").
+- iMod (known_alloc 2 with "unknown") as "#known".
+  iIntros "!> !>". iSplit.
+  + iIntros "#p_sk".
+    iPoseProof ("s_sk" with "p_sk") as ">#known'".
+    by iPoseProof (known_agree with "known known'") as "%".
+  + iIntros "#contra".
+    iApply "s_sk". by iDestruct "contra" as ">[]".
+- iIntros "#p_sk".
+  iPoseProof ("s_sk" with "p_sk") as ">#known".
+  by iPoseProof (unknown_known with "[$] [//]") as "[]".
+wp_pures. wp_lam. iApply twp_key.
+rewrite [term_of_senc_key]unlock /=.
+iApply ("post" $! (SEncKey _) with "[] [$] [$]").
+by rewrite minted_TKey.
+Qed.
+
+Lemma wp_mk_senc_key Ψ :
+  cryptis_ctx -∗
+  (∀ k : senc_key,
+      minted k -∗
+      secret k -∗
+      term_token k ⊤ -∗
+      Ψ k) -∗
+  WP mk_senc_key #() {{ Ψ }}.
+Proof.
+iIntros "#? ?". iApply twp_wp. by wp_apply twp_mk_senc_key.
+Qed.
+
+Lemma twp_aenc (sk : aenc_key) N t φ Ψ :
+  aenc_pred N φ -∗
+  minted sk -∗
+  minted t -∗
+  public t ∨ □ φ sk t ∧ □ (public sk → public t) -∗
+  (∀ m, public m → Ψ m) -∗
+  WP aenc (Spec.pkey sk) (Tag N) t [{ Ψ }].
+Proof.
+iIntros "#? #? #? #inv post".
+wp_lam. wp_pures. wp_apply twp_enc. iApply "post".
+iDestruct "inv" as "[p_t|[??]]".
+- iApply public_TSealIP.
+  + by iApply public_aenc_key.
+  + by rewrite public_tag.
+- iApply public_aencIS => //.
+Qed.
+
+Lemma wp_aenc (sk : aenc_key) N t φ Ψ :
+  aenc_pred N φ -∗
+  minted sk -∗
+  minted t -∗
+  public t ∨ □ φ sk t ∧ □ (public sk → public t) -∗
+  (∀ m, public m → Ψ m) -∗
+  WP aenc (Spec.pkey sk) (Tag N) t {{ Ψ }}.
+Proof.
+iIntros "#? #? #? #? ?".
+iApply twp_wp. by wp_apply twp_aenc.
+Qed.
+
+Lemma wp_adec (sk : aenc_key) N m φ Ψ :
+  aenc_pred N φ -∗
+  public m -∗
+  (∀ t, minted t -∗
+        public t ∨ □ φ sk t ∧ □ (public sk → public t) -∗
+        Ψ (SOMEV t)) ∧
+  Ψ NONEV -∗
+  WP adec sk (Tag N) m {{ Ψ }}.
+Proof.
+iIntros "#? #p_m post".
+wp_lam. wp_pure _ credit:"c". wp_pures. iApply wp_fupd. wp_apply wp_dec.
+case: Spec.decP => [k_t t /Spec.open_key_aencK -> ->|]; last first.
+{ iDestruct "post" as "[_ post]". iApply "post". }
+iPoseProof (public_aencE with "p_m [//]") as "[? [p_t|[#inv #p_t]]]".
+- iApply "post" => //. by eauto.
+- iMod (lc_fupd_elim_later_pers with "c inv") as "#?".
+  iApply "post" => //. by eauto.
+Qed.
+
+Lemma twp_senc (sk : senc_key) N t φ Ψ :
+  senc_pred N φ -∗
+  minted sk -∗
+  minted t -∗
+  public sk ∨ □ φ sk t -∗
+  □ (public sk → public t) -∗
+  (∀ m, public m → Ψ m) -∗
+  WP senc sk (Tag N) t [{ Ψ }].
+Proof.
+iIntros "#? #? #? #inv #p_t post".
+wp_lam. wp_pures. wp_apply twp_enc. iApply "post".
+iDestruct "inv" as "[p_sk|inv]".
+- iApply public_TSealIP => //.
+  rewrite public_tag. by iApply "p_t".
+- by iApply public_sencIS => //.
+Qed.
+
+Lemma wp_senc (sk : senc_key) N t φ Ψ :
+  senc_pred N φ -∗
+  minted sk -∗
+  minted t -∗
+  public sk ∨ □ φ sk t -∗
+  □ (public sk → public t) -∗
+  (∀ m, public m → Ψ m) -∗
+  WP senc sk (Tag N) t {{ Ψ }}.
+Proof. by iIntros "#?#?#?#?#??"; iApply twp_wp; iApply twp_senc. Qed.
+
+Lemma wp_sdec (sk : senc_key) N m φ Ψ :
+  senc_pred N φ -∗
+  public m -∗
+  (∀ t, minted t -∗
+        public sk ∨ □ φ sk t -∗
+        □ (public sk → public t) -∗
+        Ψ (SOMEV t)) ∧
+  Ψ NONEV -∗
+  WP sdec sk (Tag N) m {{ Ψ }}.
+Proof.
+iIntros "#? #p_m post".
+wp_lam. wp_pure _ credit:"c". wp_pures. iApply wp_fupd. wp_apply wp_dec.
+case: Spec.decP => [k_t t /Spec.open_key_sencK -> ->|]; last first.
+{ iDestruct "post" as "[_ post]". iApply "post". }
+iPoseProof (public_sencE with "p_m [//]") as "(? & [p_k|inv] & #p_t)".
+- iApply "post" => //. by eauto.
+- iMod (lc_fupd_elim_later_pers with "c inv") as "#?".
+  iApply "post" => //. by eauto.
+Qed.
+
+Lemma twp_sign (sk : sign_key) N t φ Ψ :
+  sign_pred N φ -∗
+  minted sk -∗
+  public t -∗
+  public sk ∨ □ φ sk t -∗
+  (∀ m, public m → Ψ m) -∗
+  WP sign sk (Tag N) t [{ Ψ }].
+Proof.
+iIntros "#? #? #? #inv post".
+wp_lam. wp_pures. wp_apply twp_enc. iApply "post".
+iDestruct "inv" as "[p_t|#?]".
+- iApply public_TSealIP => //.
+  by rewrite public_tag.
+- by iApply public_signIS => //.
+Qed.
+
+Lemma wp_sign (sk : sign_key) N t φ Ψ :
+  sign_pred N φ -∗
+  minted sk -∗
+  public t -∗
+  public sk ∨ □ φ sk t -∗
+  (∀ m, public m → Ψ m) -∗
+  WP sign sk (Tag N) t {{ Ψ }}.
+Proof.
+iIntros "#? #? #? #? ?".
+iApply twp_wp. by wp_apply twp_sign.
+Qed.
+
+Lemma wp_verify (sk : sign_key) N m φ Ψ :
+  sign_pred N φ -∗
+  public m -∗
+  (∀ t, public t -∗
+        public sk ∨ □ φ sk t -∗
+        Ψ (SOMEV t)) ∧
+  Ψ NONEV -∗
+  WP verify (Spec.pkey sk) (Tag N) m {{ Ψ }}.
+Proof.
+iIntros "#? #p_m post".
+wp_lam. wp_pure _ credit:"c". wp_pures. iApply wp_fupd. wp_apply wp_dec.
+case: Spec.decP => [k_t t /Spec.open_key_signK -> ->|]; last first.
+{ iDestruct "post" as "[_ post]". iApply "post". }
+iPoseProof (public_signE with "p_m [//]") as "[? [p_t|#inv]]".
+- iApply "post" => //. by eauto.
+- iMod (lc_fupd_elim_later_pers with "c inv") as "#?".
+  iApply "post" => //. by eauto.
+Qed.
+
+Lemma twp_is_aenc_key pk Ψ :
+  minted pk -∗
+  (∀ sk : aenc_key, ⌜pk = Spec.pkey sk⌝ -∗ minted sk -∗ Ψ #true) ∧ Ψ #false -∗
+  WP is_aenc_key pk [{ Ψ }].
+Proof.
+iIntros "#m_pk post".
+wp_lam. wp_apply (twp_has_key_type AEnc).
+case: pk; try by move=> *; iDestruct "post" as "[_ post]".
+move=> kt t.
+case: kt; try by iDestruct "post" as "[_ post]".
+iDestruct "post" as "[post _]".
+by iApply ("post" $! (AEncKey t)) => //;
+rewrite [term_of_aenc_key]unlock // !minted_TKey.
+Qed.
+
+Lemma wp_is_aenc_key pk Ψ :
+  minted pk -∗
+  (∀ sk : aenc_key, ⌜pk = Spec.pkey sk⌝ -∗ minted sk -∗ Ψ #true) ∧ Ψ #false -∗
+  WP is_aenc_key pk {{ Ψ }}.
+Proof.
+by iIntros "H1 H2"; iApply twp_wp;
+iApply (twp_is_aenc_key with "H1 H2").
+Qed.
+
+Lemma twp_is_adec_key sk Ψ :
+  minted sk -∗
+  (∀ sk' : aenc_key, ⌜sk = sk'⌝ -∗ Ψ #true) ∧ Ψ #false -∗
+  WP is_adec_key sk [{ Ψ }].
+Proof.
+iIntros "#m_pk post".
+wp_lam. wp_apply (twp_has_key_type ADec).
+case: sk; try by move=> *; iDestruct "post" as "[_ post]".
+move=> kt t.
+case: kt; try by iDestruct "post" as "[_ post]".
+iDestruct "post" as "[post _]".
+by iApply ("post" $! (AEncKey t)) => //;
+rewrite [term_of_aenc_key]unlock // !minted_TKey.
+Qed.
+
+Lemma wp_is_adec_key sk Ψ :
+  minted sk -∗
+  (∀ sk' : aenc_key, ⌜sk = sk'⌝ -∗ Ψ #true) ∧ Ψ #false -∗
+  WP is_adec_key sk {{ Ψ }}.
+Proof.
+by iIntros "H1 H2"; iApply twp_wp;
+iApply (twp_is_adec_key with "H1 H2").
+Qed.
+
+Lemma twp_is_senc_key k Ψ :
+  minted k -∗
+  (∀ k' : senc_key, ⌜k = k'⌝ -∗ Ψ #true) ∧ Ψ #false -∗
+  WP is_senc_key k [{ Ψ }].
+Proof.
+iIntros "#m_pk post".
+wp_lam. wp_apply (twp_has_key_type SEnc).
+case: k; try by move=> *; iDestruct "post" as "[_ post]".
+move=> kt t.
+case: kt; try by iDestruct "post" as "[_ post]".
+iDestruct "post" as "[post _]".
+by iApply ("post" $! (SEncKey t)) => //;
+rewrite [term_of_senc_key]unlock // !minted_TKey.
+Qed.
+
+Lemma wp_is_senc_key k Ψ :
+  minted k -∗
+  (∀ k' : senc_key, ⌜k = k'⌝ -∗ Ψ #true) ∧ Ψ #false -∗
+  WP is_senc_key k {{ Ψ }}.
+Proof.
+by iIntros "H1 H2"; iApply twp_wp;
+iApply (twp_is_senc_key with "H1 H2").
+Qed.
+
+Lemma twp_is_verify_key pk Ψ :
+  minted pk -∗
+  (∀ sk : sign_key, ⌜pk = Spec.pkey sk⌝ -∗ minted sk -∗ Ψ #true) ∧ Ψ #false -∗
+  WP is_verify_key pk [{ Ψ }].
+Proof.
+iIntros "#m_pk post".
+wp_lam. wp_apply (twp_has_key_type Verify).
+case: pk; try by move=> *; iDestruct "post" as "[_ post]".
+move=> kt t.
+case: kt; try by iDestruct "post" as "[_ post]".
+iDestruct "post" as "[post _]".
+by iApply ("post" $! (SignKey t)) => //;
+rewrite [term_of_sign_key]unlock // !minted_TKey.
+Qed.
+
+Lemma wp_is_verify_key pk Ψ :
+  minted pk -∗
+  (∀ sk : sign_key, ⌜pk = Spec.pkey sk⌝ -∗ minted sk -∗ Ψ #true) ∧ Ψ #false -∗
+  WP is_verify_key pk {{ Ψ }}.
+Proof.
+by iIntros "H1 H2"; iApply twp_wp;
+iApply (twp_is_verify_key with "H1 H2").
+Qed.
+
+Lemma twp_is_sign_key sk Ψ :
+  minted sk -∗
+  (∀ sk' : sign_key, ⌜sk = sk'⌝ -∗ Ψ #true) ∧ Ψ #false -∗
+  WP is_sign_key sk [{ Ψ }].
+Proof.
+iIntros "#m_pk post".
+wp_lam. wp_apply (twp_has_key_type Sign).
+case: sk; try by move=> *; iDestruct "post" as "[_ post]".
+move=> kt t.
+case: kt; try by iDestruct "post" as "[_ post]".
+iDestruct "post" as "[post _]".
+by iApply ("post" $! (SignKey t)) => //;
+rewrite [term_of_sign_key]unlock // !minted_TKey.
+Qed.
+
+Lemma wp_is_sign_key sk Ψ :
+  minted sk -∗
+  (∀ sk' : sign_key, ⌜sk = sk'⌝ -∗ Ψ #true) ∧ Ψ #false -∗
+  WP is_sign_key sk {{ Ψ }}.
+Proof.
+by iIntros "H1 H2"; iApply twp_wp;
+iApply (twp_is_sign_key with "H1 H2").
+Qed.
+
+End Proofs.
+
+Arguments channel {Σ _ _} c.
